### Separate Catalog TTL file

<http://fdp.com/catalog/33d0d435-4490-4bce-882a-e66d6f0b49c3>
    a  dcat:Catalog
    dct:title "{catalogue.title}" ;
    dct:isPartOf <http://fdp.com> ;
    dcat:dataset <http://fdp.com/dataset/81cf0c41-faf6-4ef4-858c-c6ed8d528826> 
    . 

### Separate Dataset TTL file

# Proposition one :
<http://fdp.com/dataset/81cf0c41-faf6-4ef4-858c-c6ed8d528826> 
    a dcat:Dataset ;
    dcterms:title "{dataset.title}" ; 
    dct:hasVersion "{dataset.version}" ;
    dct:description "{dataset.description}" ;
    dct:isPartOf <http://fdp.com/catalog/33d0d435-4490-4bce-882a-e66d6f0b49c3>;
    dqv:hasQualityAnnotation <http://fdp.com/qualityCertificate/2158d86b-7b1d-4955-a1e7-c70fb58f7f16>
    .


### Separate Quality certificate TTL file

<http://fdp.com/qualityCertificate/2158d86b-7b1d-4955-a1e7-c70fb58f7f16> 
    a dqv:QualityCertificate ;
    oa:hasTarget <http://fdp.com/dataset/81cf0c41-faf6-4ef4-858c-c6ed8d528826> ; #dct: ispartof
    dct:isPartOf <http://fdp.com/dataset/81cf0c41-faf6-4ef4-858c-c6ed8d528826> ;
    oa:hasBody :three_stars ;
    dct:title "Quality label 1"@en, "Label Qualit√© 1"@fr ;  # for FDP constraint purpose  
    oa:motivatedBy dqv:qualityAssessment
    dqv:inDimension 
        :accessability,
        :populationCoverage,
        :populationRepresentativity,
        :compliance,
        :dataProvenance,
        :metadataScope,
        :accuracy,
        :coherence,
        :completeness,
        :consistency,
        :precision,
        :validity
    .

# Definition of the OpenData5Star concept scheme
:CustomQuantumQuality
    a skos:ConceptScheme ;
    skos:prefLabel "Quantum Data Quality"@en ;
    skos:definition "A rating system used to evaluate Dataset Data qyality within the QUANTUM framework"@en 
    .

# Additional star levels for completeness
:one_star
    a skos:Concept ;
    skos:inScheme :CustomQuantumQuality ;
    skos:prefLabel "One star"@en ;
    skos:definition "MEDIAN Dataset quality of 25%"@en 
    .

:two_stars
    a skos:Concept ;
    skos:inScheme :CustomQuantumQuality ;
    skos:prefLabel "Two stars"@en ;
    skos:definition "MEDIAN Dataset quality of 45%"@en 
    .

:three_stars
    a skos:Concept ;
    skos:inScheme :CustomQuantumQuality ;
    skos:prefLabel "Three stars"@en ;
    skos:definition "MEDIAN Dataset quality of 60%"@en 

    .

:four_stars
    a skos:Concept ;
    skos:inScheme :CustomQuantumQuality ;
    skos:prefLabel "Four stars"@en ;
    skos:definition "MEDIAN Dataset quality of 80%"@en 
    .

:five_stars
    a skos:Concept ;
    skos:inScheme :CustomQuantumQuality ;
    skos:prefLabel "Five stars"@en ;
    skos:definition "MEDIAN Dataset quality of 90%"@en 
    .


<http://fdp.com/dataset/81cf0c41-faf6-4ef4-858c-c6ed8d528826>
    a dcat:Dataset ;
    dqv:hasQualityMeasurement 
        :accessibility_measurement1, 
        :accessibility_measurement2,
        :populationCoverage_measurement1,
        :populationRepresentativity_measurement1,
        :compliance_measurement1,
        :dataProvenance_measurement1,
        :dataProvenance_measurement2,
        :metadataScope_measurement1,
        :metadataScope_measurement2,
        :accuracy_measurement1,
        :coherence_measurement1,
        :completeness_measurement1, 
        :consistency_measurement1,
        :precision_measurement1,
        :validity_measurement1
    .

:accessibility_measurement1
    a dqv:QualityMeasurement ;
    dqv:computedOn : <http://fdp.com/dataset/81cf0c41-faf6-4ef4-858c-c6ed8d528826> ;
    dqv:isMeasurementOf :accessibility_metric1 ;
    dqv:value "metric_value.value"^^xsd:decimal 
    .

:accessibility_measurement2
    a dqv:QualityMeasurement ;
    dqv:computedOn : <http://fdp.com/dataset/81cf0c41-faf6-4ef4-858c-c6ed8d528826> ;
    dqv:isMeasurementOf :accessibility_metric2;
    dqv:value "metric_value.value"^^xsd:decimal 
    .

:populationCoverage_measurement1
    a dqv:QualityMeasurement ;
    dqv:computedOn : <http://fdp.com/dataset/81cf0c41-faf6-4ef4-858c-c6ed8d528826> ;
    dqv:isMeasurementOf :populationCoverage_metric1;
    dqv:value "metric_value.value"^^xsd:decimal 
    .

:populationRepresentativity_measurement1
    a dqv:QualityMeasurement ;
    dqv:computedOn : <http://fdp.com/dataset/81cf0c41-faf6-4ef4-858c-c6ed8d528826> ;
    dqv:isMeasurementOf :populationRepresentativity_measurement1;
    dqv:value "metric_value.value"^^xsd:decimal 
    .

:compliance_measurement1
    a dqv:QualityMeasurement ;
    dqv:computedOn : <http://fdp.com/dataset/81cf0c41-faf6-4ef4-858c-c6ed8d528826> ;
    dqv:isMeasurementOf :compliance_metric1;
    dqv:value "metric_value.value"^^xsd:decimal 
    .

:dataProvenance_measurement1
    a dqv:QualityMeasurement ;
    dqv:computedOn : <http://fdp.com/dataset/81cf0c41-faf6-4ef4-858c-c6ed8d528826> ;
    dqv:isMeasurementOf :dataProvenance_metric1;
    dqv:value "metric_value.value"^^xsd:decimal 
    .

:dataProvenance_measurement2
    a dqv:QualityMeasurement ;
    dqv:computedOn : <http://fdp.com/dataset/81cf0c41-faf6-4ef4-858c-c6ed8d528826> ;
    dqv:isMeasurementOf :dataProvenance_metric2;
    dqv:value "metric_value.value"^^xsd:decimal 
    .

:metadataScope_measurement1
    a dqv:QualityMeasurement ;
    dqv:computedOn : <http://fdp.com/dataset/81cf0c41-faf6-4ef4-858c-c6ed8d528826> ;
    dqv:isMeasurementOf :metadataScope_metric1;
    dqv:value "metric_value.value"^^xsd:decimal 
    .

:metadataScope_measurement2
    a dqv:QualityMeasurement ;
    dqv:computedOn : <http://fdp.com/dataset/81cf0c41-faf6-4ef4-858c-c6ed8d528826> ;
    dqv:isMeasurementOf :metadataScope_metric2;
    dqv:value "metric_value.value"^^xsd:decimal 
    .

:accuracy_measurement1
    a dqv:QualityMeasurement ;
    dqv:computedOn : <http://fdp.com/dataset/81cf0c41-faf6-4ef4-858c-c6ed8d528826> ;
    dqv:isMeasurementOf :accuracy_metric1;
    dqv:value "metric_value.value"^^xsd:decimal 
    .

:coherence_measurement1
    a dqv:QualityMeasurement ;
    dqv:computedOn : <http://fdp.com/dataset/81cf0c41-faf6-4ef4-858c-c6ed8d528826> ;
    dqv:isMeasurementOf :coherence_metric1;
    dqv:value "metric_value.value"^^xsd:decimal 
    .

:completeness_measurement1
    a dqv:QualityMeasurement ;
    dqv:computedOn : <http://fdp.com/dataset/81cf0c41-faf6-4ef4-858c-c6ed8d528826> ;
    dqv:isMeasurementOf :completeness_metric1;
    dqv:value "metric_value.value"^^xsd:decimal 
    .

:consistency_measurement1
    a dqv:QualityMeasurement ;
    dqv:computedOn : <http://fdp.com/dataset/81cf0c41-faf6-4ef4-858c-c6ed8d528826> ;
    dqv:isMeasurementOf :consistency_metric1;
    dqv:value "metric_value.value"^^xsd:decimal 
    .

:precision_measurement1
    a dqv:QualityMeasurement ;
    dqv:computedOn : <http://fdp.com/dataset/81cf0c41-faf6-4ef4-858c-c6ed8d528826> ;
    dqv:isMeasurementOf :precision_metric1;
    dqv:value "metric_value.value"^^xsd:decimal 
    .

:validity_measurement1
    a dqv:QualityMeasurement ;
    dqv:computedOn : <http://fdp.com/dataset/81cf0c41-faf6-4ef4-858c-c6ed8d528826> ;
    dqv:isMeasurementOf :validity_metric1;
    dqv:value "metric_value.value"^^xsd:decimal 
    .

-------------------------------------------------# here are the info of the metrics
:accessibility_metric1 
    a dqv:Metric ;
    skos:definition "Availability of a data access & usage policy at the time of release of the dataset"
    dereferenceable."@en ;
    dqv:expectedDataType xsd:string ; #we have categorical values
    dqv:inDimension :accessability
    .

:accessibility_metric2
    a dqv:Metric ; 	
    skos:definition "Average time from data access application to data release for a specific dataset"
    scope."@en ;
    dqv:expectedDataType xsd:string ;
    dqv:inDimension :accessability
    .

:populationCoverage_metric1
    a dqv:Metric ;
    skos:definition "Coverage Rate (percentage of the eligible population represented in the dataset)"
    dereferenceable."@en ;
    dqv:expectedDataType xsd:string ; 
    dqv:inDimension :populationCoverage

:populationRepresentativity_metric1
    a dqv:Metric ;
    skos:definition "How closely does the observed population represent the expected population?"
    dereferenceable."@en ;
    dqv:expectedDataType xsd:string ; 
    dqv:inDimension :populationRepresentativity

:compliance_metric1
    a dqv:Metric ;
    skos:definition "Is there documentation of compliance with ethical standards, conventions, protocols or regulations?"
    dereferenceable."@en ;
    dqv:expectedDataType xsd:string ; 
    dqv:inDimension :compliance

:dataProvenance_metric1
    a dqv:Metric ;
    skos:definition "Is the source of the dataset documented?"
    dereferenceable."@en ;
    dqv:expectedDataType xsd:string ; 
    dqv:inDimension :dataProvenance

:dataProvenance_metric2
    a dqv:Metric ;
    skos:definition "Are the processes and operations on the data documented?"
    dereferenceable."@en ;
    dqv:expectedDataType xsd:string ; 
    dqv:inDimension :dataProvenance

:metadataScope_metric1
    a dqv:Metric ;
    skos:definition "Existence of comprehensive standardised metadata"
    dereferenceable."@en ;
    dqv:expectedDataType xsd:string ; 
    dqv:inDimension :metadataScope

:metadataScope_metric2
    a dqv:Metric ;
    skos:definition "Existence of an exhaustive data dictionary at variable level"
    dereferenceable."@en ;
    dqv:expectedDataType xsd:string ; 
    dqv:inDimension :metadataScope

:accuracy_metric1
    a dqv:Metric ;
    skos:definition "Is accuracy of the dataset documented?"
    dereferenceable."@en ;
    dqv:expectedDataType xsd:string ; 
    dqv:inDimension :accuracy

:coherence_metric1
    a dqv:Metric ;
    skos:definition "Is coherence of the dataset documented?"
    dereferenceable."@en ;
    dqv:expectedDataType xsd:string ; 
    dqv:inDimension :coherence
    
:completeness_metric1
    a dqv:Metric ;
    skos:definition "Is completeness of the dataset documented?"
    dereferenceable."@en ;
    dqv:expectedDataType xsd:string ; 
    dqv:inDimension :completeness  

:consistency_metric1
    a dqv:Metric ;
    skos:definition "Is consistency of the dataset documented?"
    dereferenceable."@en ;
    dqv:expectedDataType xsd:string ; 
    dqv:inDimension :consistency     

:precision_metric1
    a dqv:Metric ;
    skos:definition "Is precision of the dataset documented?"
    dereferenceable."@en ;
    dqv:expectedDataType xsd:string ; 
    dqv:inDimension :precision     

:validity_metric1
    a dqv:Metric ;
    skos:definition "Availability of a conformance report for the data model."
    dereferenceable."@en ;
    dqv:expectedDataType xsd:string ; 
    dqv:inDimension :precision      


-------------------------------------------------# here are the info of the dimension
:accessability
    a dqv:Dimension ;
    skos:prefLabel "accessability"@en ;
    skos:definition "Accessibility refers to the dataset being accompanied by clear and transparent access and usage conditions."@en ; 
    dqv:inCategory :accessAndProvision
    .

:populationCoverage
    a dqv:Dimension ;
    skos:prefLabel "Population coverage"@en ;
    skos:definition "Population coverage refers to the degree to which a dataset includes the potential eligible population."@en ; 
    dqv:inCategory :coverage
    .

:populationRepresentativity
    a dqv:Dimension ;
    skos:prefLabel "Population representativity"@en ;
    skos:definition "Population representativity refers to the degree to which the data adequately represent the population in question."@en ; 
    dqv:inCategory :coverage
    .

:compliance
    a dqv:Dimension ;
    skos:prefLabel "Compliance"@en ;
    skos:definition "Compliance refers to the degree to which data has attributes that adhere to ethical standards, conventions, protocols or regulations."@en ; 
    dqv:inCategory :dataDocumentation
    .

:dataProvenance
    a dqv:Dimension ;
    skos:prefLabel "Data provenance"@en ;
    skos:definition "Data provenance means a description of the source of the data, including context, purpose, method and technology of data generation, documenting agents involved in the provenance of data, data validation routines, source data verification, traceability of changes, and quality control of data."@en ; 
    dqv:inCategory :dataDocumentation
    .

:metadataScope
    a dqv:Dimension ;
    skos:prefLabel "Metadata scope"@en ;
    skos:definition "Metadata scope refers to the availability, comprehensiveness, level of detail of metadata and data dictionary that help users understand the data being used."@en ; 
    dqv:inCategory :dataDocumentation
    .

:accuracy
    a dqv:Dimension ;
    skos:prefLabel "Accuracy"@en ;
    skos:definition "Accuracy refers to the degree to which observations correctly describe what it was designed to measure."@en ; 
    dqv:inCategory :technicalQuality
    .

:coherence
    a dqv:Dimension ;
    skos:prefLabel "Coherence"@en ;
    skos:definition "Coherence is defined as the dimension that expresses how different parts of the dataset are uniform in their representation and meaning over time, such as formats, semantics (stability of the data models), and methods."@en ; 
    dqv:inCategory :technicalQuality
    .

:completeness
    a dqv:Dimension ;
    skos:prefLabel "Completeness"@en ;
    skos:definition "Coherence is defined as the dimension that expresses how different parts of the dataset are uniform in their representation and meaning over time, such as formats, semantics (stability of the data models), and methods."@en ; 
    dqv:inCategory :technicalQuality
    .

:consistency
    a dqv:Dimension ;
    skos:prefLabel "Consistency"@en ;
    skos:definition "Consistency refers to the degree to which data has attributes that are plausible and are uniform with other data and over time."@en ; 
    dqv:inCategory :technicalQuality
    .

:precision
    a dqv:Dimension ;
    skos:prefLabel "Precision"@en ;
    skos:definition "Precision refers to the degree of approximation by which data can represent reality."@en ; 
    dqv:inCategory :technicalQuality
    .

:validity
    a dqv:Dimension ;
    skos:prefLabel "Validity"@en ;
    skos:definition "Validity refers to the degree to which representations of data in a dataset conform to the specification of a data model or data models."@en ; 
    dqv:inCategory :technicalQuality
    .


-------------------------------------------------#here are the info of the EHDS categories 
:accessAndProvision
    a  dqv:Category ;
    skos:prefLabel "Access and Provision"@en ;
    skos:definition "EHDS category grouping Accessibility dimension"@en 
    . 

:coverage
    a  dqv:Category ;
    skos:prefLabel "Coverage"@en ;
    skos:definition "EHDS category grouping Population coverage and Population Representativity dimensions"@en 
    . 

:dataDocumentation
    a  dqv:Category ;
    skos:prefLabel "Data documentation"@en ;
    skos:definition "EHDS category grouping Compliance, Data Provenance and Metadata Scope dimensions"@en 
    . 

:technicalQuality
    a  dqv:Category ;
    skos:prefLabel "Technical Quality"@en ;
    skos:definition "EHDS category grouping Accuracy, Coherence, Completeness, Consistency, Precision and Validity dimensions"@en 
    . 

